Lp2lc/Active/package.lean
@@ -3,5 +3,6 @@
 import «Lp2lc».Active.STLC.Def
 import «Lp2lc».Active.STLC.Scratch
 import «Lp2lc».Active.DTLC.Proof
+import «Lp2lc».Active.DTLC.Runtime
 
 import «Lp2lc».Active.DOT.Def
