Tests/DTLC/package.lean
@@ -1,3 +1,4 @@
 import Tests.DTLC.ValSpec
 import Tests.DTLC.TrmSpec
 import Tests.DTLC.TypSpec
+import Tests.DTLC.Runtime
